theories/rules/donate.v
@@ -42,12 +42,12 @@ Lemma hvc_donate_nz {instr i wi r2 pi ptx sown q sacc sexcl des qh sh} {l :Word}
   ∗ ▷ O@i:={q}[sown] ∗ ▷ A@i:={1}[sacc] ∗ ▷ E@i:={1}[sexcl]
   ∗ ▷ (R0 @@ i ->r r0) ∗ ▷ (R1 @@ i ->r r1) ∗ ▷(R2 @@i ->r r2) ∗  ▷ TX@ i := ptx
   ∗ ▷ mem_region des ptx
-  ∗ ▷ hp{ qh }[ (GSet sh)] }}}
+  ∗ ▷ hp{ qh }[ sh ] }}}
    ExecI @ i {{{ RET ExecI ; PC @@ i ->r (ai ^+ 1)%f ∗ ai ->a wi
   ∗ O@i:={q}[sown] ∗ A@i:={1}[sacc∖spsd] ∗ E@i:={1}[sexcl∖spsd]
   ∗ R0 @@ i ->r (encode_hvc_ret_code Succ) ∗ R1 @@ i ->r r1  ∗ TX@ i := ptx
   ∗ ∃(wh: Word), ( ⌜ wh ∈ sh ⌝ ∗ R2 @@ i ->r wh ∗ wh ->t{1}(i,W0, j , psd,Donation)
-  ∗ wh ->re false ∗ R2 @@ i ->r wh ∗ hp{qh}[(GSet (sh∖{[wh]}))] )
+  ∗ wh ->re false ∗ R2 @@ i ->r wh ∗ hp{qh}[ (sh∖{[wh]})] )
   ∗ mem_region des ptx}}}.
 Proof.
   iIntros (Hinstr Hdecodei Hini Hdecodef Hneq Hlenpsd Hdesc Hindesc Hlenr1 Hspsd Hsacc Hsown Hsexcl Hshne Φ ).
@@ -57,7 +57,7 @@ Proof.
   inversion Hsche as [ Hcureq ]; clear Hsche.
   apply fin_to_nat_inj in Hcureq.
   iModIntro.
-  iDestruct "Hσ" as "(Hcur & Hσmem & Hσreg & Hσtx & ? & Hσowned & Hσaccess & Hσexcl & Htrans & Hσhp & Hrcv)".
+  iDestruct "Hσ" as "(Hcur & Hσmem & Hσreg & Hσtx & ? & Hσowned & Hσaccess & Hσexcl & Htrans & Hσhp & %Hdisj & Hrcv)".
   (* valid regs *)
   iDestruct ((gen_reg_valid4 σ1 i PC ai R0 r0 R1 r1 R2 r2 Hcureq ) with "Hσreg PC R0 R1 R2 ")
     as "[%HPC [%HR0 [%HR1 %HR2]]]";eauto.
